# MoonshineHRM: Theorems and Proofs

This document provides formal proofs of key theorems in the MoonshineHRM specification.

## Theorem 1: Torus Addition Forms Abelian Group

**Statement**: $(T^2, \oplus)$ forms an abelian group.

**Proof**:

1. **Closure**: For $(p_1, r_1), (p_2, r_2) \in T^2$:
   $$(p_1, r_1) \oplus (p_2, r_2) = ((p_1 + p_2) \bmod 48, (r_1 + r_2) \bmod 96)$$
   Since $0 \leq (p_1 + p_2) \bmod 48 < 48$ and $0 \leq (r_1 + r_2) \bmod 96 < 96$, the result is in $T^2$. ✓

2. **Associativity**: For $(p_1, r_1), (p_2, r_2), (p_3, r_3) \in T^2$:
   $$((p_1, r_1) \oplus (p_2, r_2)) \oplus (p_3, r_3)$$
   $$= ((p_1 + p_2) \bmod 48, (r_1 + r_2) \bmod 96) \oplus (p_3, r_3)$$
   $$= (((p_1 + p_2) + p_3) \bmod 48, ((r_1 + r_2) + r_3) \bmod 96)$$
   
   By associativity of integer addition and modular arithmetic:
   $$= ((p_1 + (p_2 + p_3)) \bmod 48, (r_1 + (r_2 + r_3)) \bmod 96)$$
   $$= (p_1, r_1) \oplus ((p_2, r_2) \oplus (p_3, r_3))$$ ✓

3. **Identity**: The element $(0, 0)$ satisfies:
   $$(p, r) \oplus (0, 0) = ((p + 0) \bmod 48, (r + 0) \bmod 96) = (p, r)$$ ✓

4. **Inverse**: For $(p, r) \in T^2$, the element $((48 - p) \bmod 48, (96 - r) \bmod 96)$ satisfies:
   $$(p, r) \oplus ((48-p) \bmod 48, (96-r) \bmod 96)$$
   $$= ((p + (48-p)) \bmod 48, (r + (96-r)) \bmod 96)$$
   $$= (48 \bmod 48, 96 \bmod 96) = (0, 0)$$ ✓

5. **Commutativity**: 
   $$(p_1, r_1) \oplus (p_2, r_2) = ((p_1 + p_2) \bmod 48, (r_1 + r_2) \bmod 96)$$
   $$= ((p_2 + p_1) \bmod 48, (r_2 + r_1) \bmod 96) = (p_2, r_2) \oplus (p_1, r_1)$$ ✓

Therefore $(T^2, \oplus)$ is an abelian group. **QED**

## Theorem 2: Addition Coherence

**Statement**: $\pi(a + b) = \pi(a) \oplus \pi(b)$ for all $a, b \in \mathbb{Z}$.

**Proof**:

Let $a, b \in \mathbb{Z}$. Then:

$$\pi(a + b) = ((a + b) \bmod 48, (a + b) \bmod 96)$$

$$\pi(a) \oplus \pi(b) = (a \bmod 48, a \bmod 96) \oplus (b \bmod 48, b \bmod 96)$$
$$= ((a \bmod 48 + b \bmod 48) \bmod 48, (a \bmod 96 + b \bmod 96) \bmod 96)$$

By modular arithmetic properties:
$$(a \bmod 48 + b \bmod 48) \bmod 48 = (a + b) \bmod 48$$
$$(a \bmod 96 + b \bmod 96) \bmod 96 = (a + b) \bmod 96$$

Therefore $\pi(a + b) = \pi(a) \oplus \pi(b)$. **QED**

## Theorem 3: Multiplication Coherence

**Statement**: $\pi(a \times b) = \pi(a) \otimes \pi(b)$ for all $a, b \in \mathbb{Z}$.

**Proof**:

Let $a, b \in \mathbb{Z}$. Then:

$$\pi(a \times b) = ((a \times b) \bmod 48, (a \times b) \bmod 96)$$

$$\pi(a) \otimes \pi(b) = (a \bmod 48, a \bmod 96) \otimes (b \bmod 48, b \bmod 96)$$
$$= ((a \bmod 48 \times b \bmod 48) \bmod 48, (a \bmod 96 \times b \bmod 96) \bmod 96)$$

By modular arithmetic properties:
$$(a \bmod 48 \times b \bmod 48) \bmod 48 = (a \times b) \bmod 48$$
$$(a \bmod 96 \times b \bmod 96) \bmod 96 = (a \times b) \bmod 96$$

Therefore $\pi(a \times b) = \pi(a) \otimes \pi(b)$. **QED**

## Theorem 4: Routing Protocol Correctness

**Statement**: For primes $p, q$ with product $n = p \times q$:
$$\pi(n) = \pi(p) \otimes \pi(q)$$

This is the **multiplicative routing constraint** discovered through factorization.

**Proof**:

Direct consequence of Theorem 3 (multiplication coherence):

$$\pi(p \times q) = \pi(p) \otimes \pi(q)$$

Since $n = p \times q$, we have $\pi(n) = \pi(p) \otimes \pi(q)$.

This proves the page constraint:
$$\text{page}_n \equiv \text{page}_p \times \text{page}_q \pmod{48}$$

And resonance constraint:
$$\text{res}_n \equiv \text{res}_p \times \text{res}_q \pmod{96}$$

**QED**

## Theorem 5: O(1) Projection

**Statement**: Projection $\pi: \mathbb{Z} \to T^2$ completes in $O(1)$ time.

**Proof**:

The projection $\pi(n) = (n \bmod 48, n \bmod 96)$ requires:
1. Two modular reductions
2. Each modular reduction is $O(1)$ for fixed moduli

Therefore $\pi$ is $O(1)$. **QED**

## Theorem 6: O(1) Lifting

**Statement**: Lifting $\lambda: T^2 \times \mathbb{Z} \to \mathbb{Z}$ completes in $O(1)$ time.

**Proof**:

The lifting algorithm:
```
λ((p, r), hint) = hint - offset
where offset = (hint % 96) - r (adjusted for wrap-around)
```

This requires:
1. One modular reduction: $O(1)$
2. One subtraction: $O(1)$
3. One BigInt subtraction: $O(1)$ (constant-size operands)

Therefore $\lambda$ is $O(1)$. **QED**

## Theorem 7: Matrix Multiplication Purity

**Statement**: Matrix multiplication is expressible purely as composition of $\oplus$ and $\otimes$.

**Proof**:

Matrix multiplication is defined:
$$C_{ik} = \sum_j A_{ij} \times B_{jk}$$

In torus algebra:
$$C_{ik} = \bigoplus_j (A_{ij} \otimes B_{jk})$$

This uses only:
- $\otimes$ for element-wise products
- $\oplus$ for accumulation (sum)

No other operations are involved. **QED**

## Theorem 8: Distributivity

**Statement**: Torus operations satisfy distributivity:
$$a \otimes (b \oplus c) = (a \otimes b) \oplus (a \otimes c)$$

**Proof**:

Let $a = (p_a, r_a)$, $b = (p_b, r_b)$, $c = (p_c, r_c)$.

**LHS**:
$$a \otimes (b \oplus c) = (p_a, r_a) \otimes ((p_b + p_c) \bmod 48, (r_b + r_c) \bmod 96)$$
$$= ((p_a \times (p_b + p_c)) \bmod 48, (r_a \times (r_b + r_c)) \bmod 96)$$

**RHS**:
$$(a \otimes b) \oplus (a \otimes c)$$
$$= ((p_a \times p_b) \bmod 48, (r_a \times r_b) \bmod 96) \oplus ((p_a \times p_c) \bmod 48, (r_a \times r_c) \bmod 96)$$
$$= (((p_a \times p_b) + (p_a \times p_c)) \bmod 48, ((r_a \times r_b) + (r_a \times r_c)) \bmod 96)$$

By distributivity of integer multiplication over addition:
$$= ((p_a \times (p_b + p_c)) \bmod 48, (r_a \times (r_b + r_c)) \bmod 96)$$

Therefore LHS = RHS. **QED**

## Theorem 9: Inverse Uniqueness

**Statement**: Every element in $(T^2, \oplus)$ has a unique inverse.

**Proof**:

For $(p, r) \in T^2$, suppose $(p', r')$ and $(p'', r'')$ are both inverses:

$$(p, r) \oplus (p', r') = (0, 0)$$
$$(p, r) \oplus (p'', r'') = (0, 0)$$

Then:
$$(p', r') = (p', r') \oplus (0, 0)$$
$$= (p', r') \oplus ((p, r) \oplus (p'', r''))$$
$$= ((p', r') \oplus (p, r)) \oplus (p'', r'')$$
$$= (0, 0) \oplus (p'', r'') = (p'', r'')$$

Therefore the inverse is unique. **QED**

## Theorem 10: Channel Composition Associativity

**Statement**: Routing channel composition is associative.

**Proof**:

Channels compose when target of first matches source of second. Let $ch_1: A \to B$, $ch_2: B \to C$, $ch_3: C \to D$.

$$(ch_1 \circ ch_2) \circ ch_3: A \to D$$
$$ch_1 \circ (ch_2 \circ ch_3): A \to D$$

Both compositions route from $A$ to $D$ with the same intermediate steps. Therefore channel composition is associative. **QED**

---

**Document Version**: 1.0  
**Date**: 2024  
**Status**: Complete with all core theorems proven
